refactor

steel/Veritas.Steel.HashAccumulator.fst
@@ -25,8 +25,7 @@ let xor_bytes (s1: Seq.seq U8.t)
   = Seq.init (Seq.length s1)
              (fun i -> Seq.index s1 i `FStar.UInt8.logxor` Seq.index s2 i)
 
-let elseq a (n:nat) = Ghost.erased (Seq.lseq a n)
-let elbytes n = elseq U8.t n
+let elbytes n = A.elseq U8.t n
 
 let exor_bytes #l (s1 s2:elbytes l)
   : elbytes l
@@ -37,7 +36,6 @@ let aggregate_hash_value (h0 h1: hash_value_t)
   = xor_bytes h0 h1
 
 let create_in (_:unit) = A.malloc 0uy 32ul
-//open FStar.Ghost
 
 let exor_bytes_pfx #l (s1 s2:elbytes l) (i:nat { i <= l })
   : elbytes l
@@ -45,53 +43,53 @@ let exor_bytes_pfx #l (s1 s2:elbytes l) (i:nat { i <= l })
       (exor_bytes #i (Seq.slice s1 0 i) (Seq.slice s2 0 i))
       (Seq.slice s1 i (Seq.length s1))
 
-assume
-val varray_pts_to (#t:Type) (a:A.array t) (x:elseq t (A.length a)) : vprop
+// assume
+// val varray_pts_to (#t:Type) (a:A.array t) (x:elseq t (A.length a)) : vprop
 
-assume
-val intro_varray_pts_to (#t:_)
-                        (#opened:inames)
-                        (a:A.array t)
-  : AT.SteelGhost (elseq t (A.length a)) opened
-    (A.varray a)
-    (fun x -> varray_pts_to a x)
-    (requires fun _ -> True)
-    (ensures fun h0 x h1 ->
-      Ghost.reveal x == A.asel a h0)
+// assume
+// val intro_varray_pts_to (#t:_)
+//                         (#opened:inames)
+//                         (a:A.array t)
+//   : AT.SteelGhost (elseq t (A.length a)) opened
+//     (A.varray a)
+//     (fun x -> varray_pts_to a x)
+//     (requires fun _ -> True)
+//     (ensures fun h0 x h1 ->
+//       Ghost.reveal x == A.asel a h0)
 
-assume
-val elim_varray_pts_to (#t:_)
-                       (#opened:inames)
-                       (a:A.array t)
-                       (c:elseq t (A.length a))
-  : AT.SteelGhost unit opened
-    (varray_pts_to a c)
-    (fun _ -> A.varray a)
-    (requires fun _ -> True)
-    (ensures fun _ _ h1 ->
-      A.asel a h1 == Ghost.reveal c)
+// assume
+// val elim_varray_pts_to (#t:_)
+//                        (#opened:inames)
+//                        (a:A.array t)
+//                        (c:elseq t (A.length a))
+//   : AT.SteelGhost unit opened
+//     (varray_pts_to a c)
+//     (fun _ -> A.varray a)
+//     (requires fun _ -> True)
+//     (ensures fun _ _ h1 ->
+//       A.asel a h1 == Ghost.reveal c)
 
-assume
-val read_pt (#t:_)
-            (a:A.array t)
-            (#r:elseq t (A.length a))
-            (i:U32.t { U32.v i < A.length a })
-  : Steel t
-    (varray_pts_to a r)
-    (fun _ -> varray_pts_to a r)
-    (requires fun _ -> True)
-    (ensures fun h0 v h1 ->
-      v == Seq.index r (U32.v i))
+// assume
+// val read_pt (#t:_)
+//             (a:A.array t)
+//             (#r:elseq t (A.length a))
+//             (i:U32.t { U32.v i < A.length a })
+//   : Steel t
+//     (varray_pts_to a r)
+//     (fun _ -> varray_pts_to a r)
+//     (requires fun _ -> True)
+//     (ensures fun h0 v h1 ->
+//       v == Seq.index r (U32.v i))
 
-assume
-val write_pt (#t:_)
-            (a:A.array t)
-            (#r:elseq t (A.length a))
-            (i:U32.t { U32.v i < A.length a })
-            (v:t)
-  : SteelT unit
-    (varray_pts_to a r)
-    (fun _ -> varray_pts_to a (Seq.upd r (U32.v i) v))
+// assume
+// val write_pt (#t:_)
+//             (a:A.array t)
+//             (#r:elseq t (A.length a))
+//             (i:U32.t { U32.v i < A.length a })
+//             (v:t)
+//   : SteelT unit
+//     (varray_pts_to a r)
+//     (fun _ -> varray_pts_to a (Seq.upd r (U32.v i) v))
 
 let ehash_value_t = elbytes 32
 
@@ -108,7 +106,7 @@ let extend_ehash_value (s1 s2:ehash_value_t) (i:nat { i < 32 })
   = ()
 
 let hpts_to (x:hash_value_buf) (s:ehash_value_t) =
-  varray_pts_to x s
+  A.varray_pts_to x s
 
 let read_hbuf (#s:ehash_value_t) (x:hash_value_buf) (i:U32.t{U32.v i < 32})
   : Steel U8.t
@@ -117,14 +115,14 @@ let read_hbuf (#s:ehash_value_t) (x:hash_value_buf) (i:U32.t{U32.v i < 32})
     (requires fun _ -> True)
     (ensures fun _ v _ ->
       v == Seq.index s (U32.v i))
-  = let v = read_pt x i in AT.return v
+  = let v = A.read_pt x i in AT.return v
 
 let write_hbuf (#s:ehash_value_t) (x:hash_value_buf) (i:U32.t{U32.v i < 32}) (v:U8.t)
   : SteelT unit
     (hpts_to x s)
     (fun _ -> hpts_to x (upd_ehash_value s (U32.v i) v))
-  = write_pt x i v;
-    AT.change_equal_slprop (varray_pts_to _ _)
+  = A.write_pt x i v;
+    AT.change_equal_slprop (A.varray_pts_to _ _)
                            (hpts_to _ _)
 
 let intro_hpts_to (#o:_) (x:hash_value_buf)
@@ -134,7 +132,7 @@ let intro_hpts_to (#o:_) (x:hash_value_buf)
     (requires fun _ -> True)
     (ensures fun h v _ ->
       as_hash_value x h == Ghost.reveal v)
-  = intro_varray_pts_to x
+  = A.intro_varray_pts_to x
 
 let elim_hpts_to (#o:_) (#e:ehash_value_t) (x:hash_value_buf)
   : AT.SteelGhost unit o
@@ -143,7 +141,7 @@ let elim_hpts_to (#o:_) (#e:ehash_value_t) (x:hash_value_buf)
     (requires fun _ -> True)
     (ensures fun _ _ h ->
       Ghost.reveal e == as_hash_value x h)
-  = elim_varray_pts_to x e
+  = A.elim_varray_pts_to x e
 
 #push-options "--query_stats --fuel 0 --ifuel 0"
 let aggregate_hash_value_pts
@@ -202,114 +200,27 @@ let aggregate_hash_value_buf (b1: hash_value_buf) (b2: hash_value_buf)
     elim_hpts_to b2
 
 
-let size_t = U32.t
-let max_output = 64
-
-assume
-val blake2b:
-    nn:size_t{1 <= UInt32.v nn /\ UInt32.v nn <= max_output}
-  -> output: A.array U8.t
-  -> ll: size_t
-  -> d: A.array U8.t
-  -> Steel unit
-  (A.varray output `star` A.varray d)
-  (fun _ -> A.varray output `star` A.varray d)
-  (requires fun _ ->
-    A.length d >= U32.v ll /\
-    A.length output = U32.v nn)
-  (ensures fun h0 _ h1 ->
-    A.length d >= U32.v ll /\
-    A.length output = U32.v nn /\
-    A.asel d h0 == A.asel d h1 /\
-    A.asel output h1 ==
-      Blake.spec
-        (Seq.slice (A.asel d h0) 0 (U32.v ll))
-        0 Seq.empty (UInt32.v nn))
-
 let add (s:hash_value_buf) (input:hashable_buffer) (l:U32.t)
   = let tmp = A.malloc 0uy 32ul in
-    blake2b 32ul tmp l input;
+    Blake.blake2b 32ul tmp l input;
     aggregate_hash_value_buf s tmp;
     A.free tmp;
     let h1 = AT.get() in //Weird to need this
     assert (A.asel s h1 == v_hash s h1);
     AT.return ()
 
-
-let coerce #t (#l0 #l1:_) (e:elseq t l0 { l0 = l1}) : elseq t l1 = e
-
-let prefix_copied #t #l0 #l1
-                  (e0:elseq t l0)
-                  (e1:elseq t l1)
-                  (i:nat { i <= l0 /\ l0 == l1})
-   : elseq t l1
-   = (Seq.append (Seq.slice e0 0 i) (Seq.slice e1 i (Seq.length e1)))
-
-let slice_lem (#t:_)
-              (#l0 #l1:_)
-              (e0:elseq t l0)
-              (e1:elseq t l1)
-  : Lemma
-    (requires l0 == l1)
-    (ensures prefix_copied e0 e1 l0 `Seq.equal`
-             coerce #t #l0 #l1 e0)
-  = ()
-
-let memcpy #t (a0 a1:A.array t)
-              (#e0:elseq t (A.length a0))
-              (#e1:elseq t (A.length a1))
-              (i:U32.t{ U32.v i == A.length a0 /\ A.length a0 == A.length a1 })
-  : SteelT unit
-    (varray_pts_to a0 e0 `star` varray_pts_to a1 e1)
-    (fun _ -> varray_pts_to a0 e0 `star` varray_pts_to a1 (coerce e0))
-  = let inv (j:Loops.nat_at_most i)
-      : vprop
-      = varray_pts_to a0 e0 `star`
-        varray_pts_to a1 (prefix_copied e0 e1 j)
-    in
-    let body (j:Loops.u32_between 0ul i)
-      : SteelT unit
-        (inv (U32.v j))
-        (fun _ -> inv (U32.v j + 1))
-      = AT.change_equal_slprop
-            (inv (U32.v j))
-            (varray_pts_to a0 e0 `star`
-             varray_pts_to a1 (prefix_copied e0 e1 (U32.v j)));
-        let z = read_pt a0 j in
-        write_pt a1 j z;
-        assert (Seq.upd (prefix_copied e0 e1 (U32.v j)) (U32.v j) z `Seq.equal`
-                prefix_copied e0 e1 (U32.v j + 1));
-        AT.change_equal_slprop (varray_pts_to a0 e0 `star` varray_pts_to a1 _)
-                               (inv (U32.v j + 1));
-        AT.return ()
-    in
-    assert (prefix_copied e0 e1 0 `Seq.equal` e1);
-    AT.change_equal_slprop (varray_pts_to a1 _)
-                           (varray_pts_to a1 (prefix_copied e0 e1 (U32.v 0ul)));
-    AT.change_equal_slprop (varray_pts_to a0 e0 `star` varray_pts_to a1 _)
-                           (inv (U32.v 0ul));
-    Loops.for_loop 0ul i inv body;
-    AT.slassert (inv (U32.v i));
-    AT.change_equal_slprop (inv (U32.v i))
-                           (varray_pts_to a0 e0 `star`
-                            varray_pts_to a1 (prefix_copied e0 e1 (U32.v i)));
-    slice_lem e0 e1;
-    AT.change_equal_slprop (varray_pts_to a1 (prefix_copied e0 e1 (U32.v i)))
-                           (varray_pts_to a1 (coerce e0));
-    AT.return ()
-
 let get' (#e0 #e1:ehash_value_t)
          (s:state)
          (out:hash_value_buf)
   : SteelT unit
-    (hpts_to s e0 `star` varray_pts_to out e1)
+    (hpts_to s e0 `star` A.varray_pts_to out e1)
     (fun _ ->
-      hpts_to s e0 `star` varray_pts_to out (coerce e0))
+      hpts_to s e0 `star` A.varray_pts_to out (A.coerce e0))
   = AT.change_equal_slprop (hpts_to s _)
-                           (varray_pts_to s e0);
-    memcpy s out 32ul;
-    AT.change_equal_slprop (varray_pts_to s _)
-                          (hpts_to s _)
+                           (A.varray_pts_to s e0);
+    A.memcpy s out 32ul;
+    AT.change_equal_slprop (A.varray_pts_to s _)
+                           (hpts_to s _)
 
 let get (s:state) (out:hash_value_buf)
   : Steel unit
@@ -320,10 +231,10 @@ let get (s:state) (out:hash_value_buf)
        v_hash s h0 == as_hash_value out h1 /\
        v_hash s h1 == v_hash s h0)
   = let _ = intro_hpts_to s in
-    let _ = intro_varray_pts_to out in
+    let _ = A.intro_varray_pts_to out in
     get' s out;
     elim_hpts_to s;
-    elim_varray_pts_to out _;
+    A.elim_varray_pts_to out _;
     AT.return ()
 
 let free (s:state) = A.free s
