steel/Veritas.Steel.Array.fst
@@ -1,0 +1,99 @@
+module Veritas.Steel.Array
+open Steel.Memory
+open Steel.Effect
+open FStar.Ghost
+module U32 = FStar.UInt32
+module A = Steel.Array
+module AT = Steel.Effect.Atomic
+module Loops = Veritas.Steel.Loops
+
+let varray_pts_to (#t:Type) (a:A.array t) (x:elseq t (A.length a))
+  : vprop
+  = admit()
+
+let intro_varray_pts_to (#t:_)
+                        (#opened:inames)
+                        (a:A.array t)
+  = AT.sladmit()
+
+let elim_varray_pts_to (#t:_)
+                       (#opened:inames)
+                       (a:A.array t)
+                       (c:elseq t (A.length a))
+  = AT.sladmit()
+
+let read_pt (#t:_)
+            (a:A.array t)
+            (#r:elseq t (A.length a))
+            (i:U32.t { U32.v i < A.length a })
+  = AT.sladmit();
+    let v = magic #t () in
+    AT.return  v
+
+
+let write_pt (#t:_)
+            (a:A.array t)
+            (#r:elseq t (A.length a))
+            (i:U32.t { U32.v i < A.length a })
+            (v:t)
+  = AT.sladmit()
+
+let prefix_copied #t #l0 #l1
+                  (e0:elseq t l0)
+                  (e1:elseq t l1)
+                  (i:nat { i <= l0 /\ l0 == l1})
+   : elseq t l1
+   = (Seq.append (Seq.slice e0 0 i) (Seq.slice e1 i (Seq.length e1)))
+
+let slice_lem (#t:_)
+              (#l0 #l1:_)
+              (e0:elseq t l0)
+              (e1:elseq t l1)
+  : Lemma
+    (requires l0 == l1)
+    (ensures prefix_copied e0 e1 l0 `Seq.equal`
+             coerce #t #l0 #l1 e0)
+  = ()
+
+let memcpy #t (a0 a1:A.array t)
+              (#e0:elseq t (A.length a0))
+              (#e1:elseq t (A.length a1))
+              (i:U32.t{ U32.v i == A.length a0 /\ A.length a0 == A.length a1 })
+  : SteelT unit
+    (varray_pts_to a0 e0 `star` varray_pts_to a1 e1)
+    (fun _ -> varray_pts_to a0 e0 `star` varray_pts_to a1 (coerce e0))
+  = let inv (j:Loops.nat_at_most i)
+      : vprop
+      = varray_pts_to a0 e0 `star`
+        varray_pts_to a1 (prefix_copied e0 e1 j)
+    in
+    let body (j:Loops.u32_between 0ul i)
+      : SteelT unit
+        (inv (U32.v j))
+        (fun _ -> inv (U32.v j + 1))
+      = AT.change_equal_slprop
+            (inv (U32.v j))
+            (varray_pts_to a0 e0 `star`
+             varray_pts_to a1 (prefix_copied e0 e1 (U32.v j)));
+        let z = read_pt a0 j in
+        write_pt a1 j z;
+        assert (Seq.upd (prefix_copied e0 e1 (U32.v j)) (U32.v j) z `Seq.equal`
+                prefix_copied e0 e1 (U32.v j + 1));
+        AT.change_equal_slprop (varray_pts_to a0 e0 `star` varray_pts_to a1 _)
+                               (inv (U32.v j + 1));
+        AT.return ()
+    in
+    assert (prefix_copied e0 e1 0 `Seq.equal` e1);
+    AT.change_equal_slprop (varray_pts_to a1 _)
+                           (varray_pts_to a1 (prefix_copied e0 e1 (U32.v 0ul)));
+    AT.change_equal_slprop (varray_pts_to a0 e0 `star` varray_pts_to a1 _)
+                           (inv (U32.v 0ul));
+    Loops.for_loop 0ul i inv body;
+    AT.slassert (inv (U32.v i));
+    AT.change_equal_slprop (inv (U32.v i))
+                           (varray_pts_to a0 e0 `star`
+                            varray_pts_to a1 (prefix_copied e0 e1 (U32.v i)));
+    slice_lem e0 e1;
+    AT.change_equal_slprop (varray_pts_to a1 (prefix_copied e0 e1 (U32.v i)))
+                           (varray_pts_to a1 (coerce e0));
+    AT.return ()
