steel/crypto/Hacl.Blake2b_32.fsti
@@ -1,66 +1,58 @@
 module Hacl.Blake2b_32
 
-// This file is here to prevent depending on the actual HACL* repository.
-// The signatures do not correspond to the ones found in the original HACL* file.
-// We assume verification good nonetheless and reconcile these files at link-time.
-//
-// In the future, we hope that the hacl-star repository will provided a minimal
-// set of fstis that allow bringing into scope the signatures (only) of the
-// various API functions of EverCrypt, all specified in terms of abstract
-// specifications.
+// This file is here to prevent depending on the actual HACL*
+// repository.  The signatures do not correspond to the ones found in
+// the original HACL* file. Notably, this is a Steel signature,
+// whereas HACL* is verified in Low*
 
-module B = LowStar.Buffer
-module ST = FStar.HyperStack.ST
+// We assume verification good nonetheless and reconcile these files
+// at link-time.
 
-#set-options "--fuel 0 --ifuel 0"
+// In the future, we hope that the hacl-star repository will provided
+// a minimal set of fstis that allow bringing into scope the
+// signatures (only) of the various API functions of EverCrypt, all
+// specified in terms of abstract specifications.
 
-// NB: this is not the definition from HACL*, since it does not rely on secret integers
-inline_for_extraction noextract
-let bytes = Seq.seq UInt8.t
+module U8 = FStar.UInt8
+module U32 = FStar.UInt32
+module A = Veritas.Steel.Array
 
-inline_for_extraction noextract
-let lbytes l = s:Seq.seq UInt8.t { Seq.length s = l }
+open Steel.Effect.Common
+open Steel.Effect
 
 inline_for_extraction noextract
 let size_nat = n:nat { n <= pow2 32 - 1 }
-
-open FStar.Mul
+let size_t = U32.t
+let max_output = 64
+let bytes = Seq.seq U8.t
 
 inline_for_extraction noextract
-let size_block = 128
+let lbytes l = s:bytes { Seq.length s = l }
 
 noextract
-val spec:
+val spec :
     d:bytes
   -> kk:size_nat{kk <= 64 /\ (if kk = 0 then Seq.length d < pow2 128 else Seq.length d + 128 < pow2 64)}
   -> k:lbytes kk
   -> nn:size_nat{1 <= nn /\ nn <= 64} ->
   Tot (lbytes nn)
 
-inline_for_extraction noextract
-let size_t = UInt32.t
-
-inline_for_extraction noextract
-let max_output = 64
-
-inline_for_extraction noextract
-let max_key = 64
-
-inline_for_extraction noextract
-let lbuffer t l = b:B.buffer t { B.len b == l }
-
 val blake2b:
     nn:size_t{1 <= UInt32.v nn /\ UInt32.v nn <= max_output}
-  -> output: lbuffer UInt8.t nn
+  -> output: A.array U8.t
   -> ll: size_t
-  -> d: lbuffer UInt8.t ll
-  -> kk: size_t{UInt32.v kk <= max_key}
-  -> k: lbuffer UInt8.t kk ->
-  ST.Stack unit
-    (requires (fun h ->
-      let open B in
-      live h output /\ live h d /\ live h k
-      /\ disjoint output d /\ disjoint output k /\ disjoint d k))
-    (ensures  (fun h0 _ h1 ->
-      B.modifies (B.loc_buffer output) h0 h1
-      /\ B.as_seq h1 output == spec (B.as_seq h0 d) (UInt32.v kk) (B.as_seq h0 k) (UInt32.v nn)))
+  -> d: A.array U8.t
+  -> Steel unit
+  (A.varray output `star` A.varray d)
+  (fun _ -> A.varray output `star` A.varray d)
+  (requires fun _ ->
+    A.length d >= U32.v ll /\
+    A.length output = U32.v nn)
+  (ensures fun h0 _ h1 ->
+    A.length d >= U32.v ll /\
+    A.length output = U32.v nn /\
+    A.asel d h0 == A.asel d h1 /\
+    A.asel output h1 ==
+      spec
+        (Seq.slice (A.asel d h0) 0 (U32.v ll))
+        0 Seq.empty (UInt32.v nn))
